add some comments

crypto_hst/symmetric/GCM.fst
@@ -22,6 +22,14 @@ type cipher_alg (k: pos) = key:u8s{length key = k} ->
     (ensures (fun h0 _ h1 -> live h1 key /\ live h1 input /\ live h1 out
         /\ modifies_1 out h0 h1))
 
+(** Every block of message is regarded as an element in Galois field GF(2^128), **)
+(** it is represented as 16 bytes. The following several functions are basic    **)
+(** operations in this field.                                                   **)
+(** gf128_add: addition. Equivalent to bitxor.                                  **)
+(** gf128_shift_right: shift right by 1 bit. Used in multiplication.            **)
+(** gf128_mul: multiplication. Achieved by combining 128 additions.             **)
+
+(* Every function "func_name_loop" is a helper for function "func_name". *)
 private val gf128_add_loop: a:u8s{length a = 16} ->
     b:u8s{length b = 16 /\ disjoint a b} ->
     dep:u32{U32.v dep <= 16} ->
@@ -38,6 +46,7 @@ let rec gf128_add_loop a b dep =
     gf128_add_loop a b i
   end
 
+(* In place addition. Calculate "a + b" and store the result in a. *)
 val gf128_add: a:u8s{length a = 16} ->
     b:u8s{length b = 16 /\ disjoint a b} ->
     STL unit
@@ -64,11 +73,13 @@ let rec gf128_shift_right_loop a dep =
     gf128_shift_right_loop a i
   end
 
+(* In place shift. Calculate "a >> 1" and store the result in a. *)
 private val gf128_shift_right: a:u8s{length a = 16} -> STL unit
     (requires (fun h -> live h a))
     (ensures (fun h0 _ h1 -> live h1 a /\ modifies_1 a h0 h1))
 let gf128_shift_right a = gf128_shift_right_loop a 15ul
 
+(* Generate mask. If the i-th bit of num is 1 then return 11111111, otherwise return 00000000. *)
 private val ith_bit_mask: num:s8 -> i:u32{U32.v i < 8} -> Tot s8
 let ith_bit_mask num i =
   let proj = shift_right (uint8_to_sint8 128uy) i in
@@ -89,6 +100,8 @@ let rec apply_mask_loop a m msk dep =
     apply_mask_loop a m msk i
   end
 
+(* This will apply a mask to each byte of u8s. *)
+(* Mask a with msk, and store the result in m. *)
 private val apply_mask: a:u8s{length a = 16} ->
     m:u8s{length m = 16 /\ disjoint a m} ->
     msk:s8 -> STL unit
@@ -122,7 +135,9 @@ let rec gf128_mul_loop a b tmp dep =
     upd a 0ul (logxor num (logand msk r_mul));
     gf128_mul_loop a b tmp (U32.add dep 1ul)
   end
-  
+
+(* In place multiplication. Calculate "a * b" and store the result in a.    *)
+(* WARNING: can only pass lax check and may have issues with constant time. *)
 val gf128_mul: a:u8s{length a = 16} ->
     b:u8s{length b = 16 /\ disjoint a b} -> STL unit
     (requires (fun h -> live h a /\ live h b))
@@ -133,7 +148,11 @@ let gf128_mul a b =
   gf128_mul_loop a b tmp 0ul;
   blit tmp 0ul a 0ul 16ul;
   pop_frame()
-  
+
+(* During authentication, the length information should also be included. *)
+(* This function will generate an element in GF128 by:                    *)
+(* 1. express len of additional data and len of ciphertext as 64-bit int; *)
+(* 2. concatenate the two integers to get a 128-bit block.                *)
 private val mk_len_info: len_info:u8s{length len_info = 16} ->
     len_1:u32 -> len_2:u32 -> STL unit
     (requires (fun h -> live h len_info))
@@ -160,6 +179,7 @@ let mk_len_info len_info len_1 len_2 =
   let len_2 = U32.shift_right len_2 8ul in
   upd len_info 11ul (uint32_to_sint8 len_2)
 
+(* WARNING: can only pass lax check and may have issues with constant time. *)
 private val ghash_loop: tag:u8s{length tag = 16} ->
     auth_key:u8s{length auth_key = 16 /\ disjoint tag auth_key} ->
     str:u8s{disjoint tag str /\ disjoint auth_key tag} ->
@@ -168,6 +188,7 @@ private val ghash_loop: tag:u8s{length tag = 16} ->
     (requires (fun h -> live h tag /\ live h auth_key /\ live h str))
     (ensures (fun h0 _ h1 -> live h1 tag /\ live h1 auth_key /\ live h1 str /\ modifies_1 tag h0 h1))
 let rec ghash_loop tag auth_key str len dep =
+  (* Appending zeros if the last block is not a complete one. *)
   if U32.gte 16ul (U32.sub len dep) then begin
     push_frame();
     let last = create (uint8_to_sint8 0uy) 16ul in
@@ -183,6 +204,9 @@ let rec ghash_loop tag auth_key str len dep =
     ghash_loop tag auth_key str len next
   end
 
+(* A hash function used in authentication. It will authenticate additional data first, *)
+(* then ciphertext and at last length information. The result is stored in tag.        *)
+(* WARNING: can only pass lax check. *)
 val ghash: auth_key:u8s{length auth_key = 16} ->
     ad:u8s{disjoint auth_key ad} ->
     adlen:u32{U32.v adlen = length ad} ->
@@ -204,6 +228,8 @@ let ghash auth_key ad adlen ciphertext len tag =
   gf128_mul tag auth_key;
   pop_frame()
 
+(* Update the counter, replace last 4 bytes of counter with num. *)
+(* num is precalculated by the function who calls this function. *)
 private val update_counter: counter:u8s{length counter = 16} ->
     num:u32 -> STL unit
     (requires (fun h -> live h counter))
@@ -217,6 +243,7 @@ let update_counter counter num =
   let num = U32.shift_right num 8ul in
   upd counter 12ul (uint32_to_sint8 num)
 
+(* WARNING: may have issues with constant time. *)
 private val auth_body: #k:pos -> alg:cipher_alg k ->
     ciphertext:u8s ->
     tag:u8s{length tag = 16 /\ disjoint ciphertext tag} ->
@@ -278,6 +305,7 @@ private val encrypt_loop: #k:pos -> alg:cipher_alg k ->
     (ensures (fun h0 _ h1 -> live h1 ciphertext /\ live h1 key /\ live h1 plaintext /\ live h1 tmp
         /\ modifies_2 ciphertext tmp h0 h1))
 let rec encrypt_loop #k alg ciphertext key cnt plaintext len tmp dep =
+  (* Appending zeros if the last block is not a complete one. *)
   if U32.gte 16ul (U32.sub len dep) then begin
     let h0 = HST.get() in
     let counter = sub tmp 0ul 16ul in
@@ -325,6 +353,8 @@ let encrypt_body #k alg ciphertext tag key nonce cnt ad adlen plaintext len =
   pop_frame();
   authenticate #k alg ciphertext tag key nonce cnt ad adlen len
 
+(** In GCM, an initialization vector is used to generate a 96-bit nonce, and can have any length. **)
+(** This version only allows 96-bit iv. This needs to be fixed.                                   **)
 val encrypt: #k:pos -> alg:cipher_alg k ->
     ciphertext:u8s ->
     tag:u8s{length tag = 16 /\ disjoint ciphertext tag} ->
@@ -340,3 +370,78 @@ val encrypt: #k:pos -> alg:cipher_alg k ->
         /\ modifies_2 ciphertext tag h0 h1))
 let encrypt #k alg ciphertext tag key iv ad adlen plaintext len =
   encrypt_body #k alg ciphertext tag key iv 1ul ad adlen plaintext len
+
+(** This is an incomplete decrypt function. The main idea is to compute tag first. **)
+(** If the result is compatible with the tag that user gives, then it will decrypt **)
+(** the ciphertext. Otherwise it will refuse to decrypt. The current GCM uses      **)
+(** encrypt function to decrypt and let the user check the tag himself.            **)
+(*
+val decrypt_body: #k:pos -> alg:cipher_alg k ->
+    plaintext:u8s ->
+    key:u8s{length key = k /\ disjoint plaintext key} ->
+    nonce:u8s{length nonce = 12 /\ disjoint plaintext nonce /\ disjoint key nonce} ->
+    cnt:u32 ->
+    ciphertext:u8s{length ciphertext = length plaintext /\ disjoint plaintext ciphertext /\ disjoint key ciphertext /\ disjoint nonce ciphertext} ->
+    len:u32{length ciphertext = U32.v len} ->
+    STL unit
+    (requires (fun h -> live h plaintext /\ live h key /\ live h nonce /\ live h ciphertext))
+    (ensures (fun h0 _ h1 -> live h1 plaintext /\ live h1 key /\ live h1 nonce /\ live h1 ciphertext
+        /\ modifies_1 plaintext h0 h1))
+let decrypt_body #k alg plaintext key nonce cnt ciphertext len =
+  push_frame();
+  let tmp = create (uint8_to_sint8 0uy) 48ul in
+  blit nonce 0ul tmp 0ul 12ul;
+  encrypt_loop #k alg plaintext key (U32.add_mod cnt 1ul) ciphertext len tmp 0ul;
+  pop_frame()
+
+val check_tag: #k:pos -> alg:cipher_alg k ->
+    ciphertext:u8s ->
+    tag:u8s{length tag = 16 /\ disjoint ciphertext tag} ->
+    key:u8s{length key = k /\ disjoint ciphertext key /\ disjoint tag key} ->
+    nonce:u8s{length nonce = 12 /\ disjoint ciphertext nonce /\ disjoint tag nonce /\ disjoint key nonce} ->
+    cnt:u32 ->
+    ad:u8s{disjoint ciphertext ad /\ disjoint tag ad /\ disjoint key ad /\ disjoint nonce ad} ->
+    adlen:u32{length ad = U32.v adlen} ->
+    len:u32{length ciphertext = U32.v len} ->
+    STL bool
+    (requires (fun h -> live h ciphertext /\ live h tag /\ live h key /\ live h nonce /\ live h ad))
+    (ensures (fun h0 _ h1 -> live h1 ciphertext /\ live h1 tag /\ live h1 key /\ live h1 nonce /\ live h1 ad
+        /\ modifies_0 h0 h1))
+let check_tag #k alg ciphertext tag key nonce cnt ad adlen len =
+  push_frame();
+  let tmp = create (uint8_to_sint8 0uy) 16ul in
+  authenticate #k alg ciphertext tmp key nonce cnt ad adlen len;
+  let res = (* Compare tmp and tag *) true in
+  pop_frame();
+  admit();
+  res
+
+val decrypt: #k:pos -> alg:cipher_alg k ->
+    plaintext:u8s ->
+    tag:u8s{length tag = 16 /\ disjoint plaintext tag} ->
+    key:u8s{length key = k /\ disjoint plaintext key /\ disjoint tag key} ->
+    iv:u8s{length iv = 12 /\ disjoint plaintext iv /\ disjoint tag iv /\ disjoint key iv} ->
+    ad:u8s{disjoint plaintext ad /\ disjoint tag ad /\ disjoint key ad /\ disjoint iv ad} ->
+    adlen:u32{length ad = U32.v adlen} ->
+    ciphertext:u8s{length ciphertext = length plaintext /\ disjoint plaintext ciphertext /\ disjoint tag ciphertext /\ disjoint key ciphertext /\ disjoint iv ciphertext /\ disjoint ad ciphertext} ->
+    len:u32{length ciphertext = U32.v len} ->
+    STL bool
+    (requires (fun h -> live h plaintext /\ live h tag /\ live h key /\ live h iv /\ live h ad /\ live h ciphertext))
+    (ensures (fun h0 r h1 -> live h1 plaintext /\ live h1 tag /\ live h1 key /\ live h1 iv /\ live h1 ad /\ live h1 ciphertext
+        /\ ((r /\ modifies_1 plaintext h0 h1) \/ ((not r) /\ modifies_0 h0 h1))))
+let decrypt #k alg plaintext tag key iv ad adlen ciphertext len =
+  let h0 = HST.get() in
+  let check = check_tag #k alg ciphertext tag key iv 1ul ad adlen len in
+  if not check then begin
+    let h1 = HST.get() in
+    assert(modifies_0 h0 h1);
+    false
+  end else begin
+    let h0' = HST.get() in
+    assert(modifies_0 h0 h0');
+    decrypt_body #k alg plaintext key iv 1ul ciphertext len;
+    let h1 = HST.get() in
+    assert(modifies_1 plaintext h0 h1);admit();
+    true
+  end
+*)
